theories/case_studies/cooperative_concurrency.v
@@ -27,7 +27,7 @@ From affect.logic Require Import tactics.
 
 (* Make all the definitions opaque so that we do not rely on their definition in the model to show that the programs are well-typed terms. *)
 Opaque sem_typed sem_typed_val ty_le row_le sig_le row_type_sub row_env_sub.
-Opaque sem_ty_void sem_ty_unit sem_ty_bool sem_ty_int sem_ty_string sem_ty_top sem_ty_bang sem_env_bang sem_ty_ref_cpy sem_ty_ref sem_ty_prod sem_ty_sum sem_ty_arr sem_ty_aarr sem_ty_uarr sem_ty_forall sem_ty_row_forall sem_ty_exists sem_ty_rec sem_ty_option sem_ty_list.
+Opaque sem_ty_void sem_ty_unit sem_ty_bool sem_ty_int sem_ty_string sem_ty_top sem_ty_bang sem_env_bang sem_ty_ref_cpy sem_ty_ref sem_ty_prod sem_ty_sum sem_ty_arr sem_ty_forall sem_ty_row_forall sem_ty_exists sem_ty_rec sem_ty_option sem_ty_list.
 Opaque sem_sig_eff sem_sig_flip_bang.
 Opaque sem_row_nil sem_row_flip_bang sem_row_cons sem_row_rec.
 
@@ -385,7 +385,7 @@ Section typing.
      + iApply (sem_typed_app_os () _ ('! β)); [iApply sem_typed_var'|]. 
        rewrite -/await_sig -/(async_sig coop) -/coop. 
        iApply sem_typed_sub_env_final; first iApply env_le_cons; first iApply env_le_refl; 
-       [iApply ty_le_aarr; try iApply ty_le_refl; iApply (row_le_rec_unfold coop_pre)|].
+       [iApply ty_le_arr; try iApply ty_le_refl; iApply (row_le_rec_unfold coop_pre)|].
        rewrite -/coop. iApply sem_typed_unit'.
      + iIntros (β').
        iApply sem_typed_swap_third. iApply sem_typed_weaken.
@@ -477,7 +477,7 @@ Section typing.
             [iApply row_le_refl|iApply ty_le_uarr|iApply ty_le_refl|];
             [iApply (row_le_mfbang_intro OS)|iApply ty_le_refl|iApply ty_le_refl|].
            iApply sem_typed_sub_ty; first iApply ty_le_uarr; 
-            [iApply row_le_refl|iApply ty_le_refl|iApply ty_le_aarr|];
+            [iApply row_le_refl|iApply ty_le_refl|iApply ty_le_arr|];
             [iApply (row_le_mfbang_elim OS)|iApply ty_le_refl|iApply ty_le_refl|].
            set C := (λ (θ : sem_row Σ), (('! β ⊸ ()) -{ ¡ θ }-> ()) → List ('! β ⊸ ()) -{ ¡ θ }-∘ ())%T.
            rewrite -/(C ⊥).
